Failed attempt at proving normalization, unclear if salvageable

theories/LambdaCube/SN.v
@@ -3,8 +3,616 @@ From Coq Require Import Arith Lia.
 From FormArith Require Import Base.
 From FormArith.LambdaCube Require Import Term Operational Typing.
 
+
 Inductive SN {n : nat} (t : term n) : Prop :=
 | SN_on : (∀ u, t ≻ u → SN u) → SN t.
+
+(* The following is an attempt at formalizing the proof of normalization for CoC
+   which can be found in Gilles Dowek's "Proofs in Theories" notes *)
+
+Notation "'𝓟' X" := (X → Prop)
+                      (at level 10,
+                       left associativity).
+
+Definition elem {X : Type} (x : X) (S : 𝓟 X) : Prop := S x.
+
+Notation "x ∈ X" := (elem x X)
+                      (at level 20,
+                         no associativity).
+
+Definition tset := ∀ (n : nat), 𝓟 (term n).
+
+Definition sn : tset := λ n t, SN t.
+
+Definition pi_set (X : tset) (S : 𝓟 tset) :=
+  λ n (t : term n),
+    SN t ∧
+    ∀ ty bod tm Y,
+       tm ∈ (X n) →
+       Y ∈ S →
+       t ≻* Abs ty bod →
+       bind (bind_first tm) bod ∈ (Y n).
+
+Definition tset_equiv (X Y : tset) : Prop :=
+  ∀ n t, X n t ↔ Y n t.
+
+Notation "X ≡ Y" := (tset_equiv X Y)
+                      (at level 20,
+                         no associativity
+                      ).
+
+Lemma tset_equiv_refl {X : tset} : X ≡ X.
+Proof. firstorder. Qed.
+
+Lemma tset_equiv_sym {X Y : tset} : X ≡ Y → Y ≡ X.
+Proof. firstorder. Qed.
+
+Lemma tset_equiv_trans {X Y Z : tset} : X ≡ Y → Y ≡ Z → X ≡ Z.
+Proof.
+  intros XY YZ n t.
+  split.
+  - intros Xt.
+    apply YZ, XY, Xt.
+  - intros Zt.
+    apply XY, YZ, Zt.
+Qed.
+
+Definition inter (S : 𝓟 tset) : tset :=
+  λ n t, ∀ Y, Y ∈ S → Y n t.
+
+Notation "⋂ S" := (inter S)
+                    (at level 10,
+                       left associativity).
+
+Inductive candidate : tset → Prop :=
+| c_sn X : X ≡ sn → candidate X
+| c_pi X S Z : Z ≡ pi_set X S →
+               candidate X →
+               (∀ Y, Y ∈ S → candidate Y) →
+               candidate Z
+| c_inter X S : X ≡ ⋂ S →
+                (∀ Y, Y ∈ S → candidate Y) →
+                candidate X.
+
+Definition Cand : Prop := ∃ X, candidate X.
+
+Definition cand_sn : Cand := ex_intro _ _ (c_sn _ tset_equiv_refl).
+
+Inductive annot : Type :=
+| sing : annot
+| c : annot
+| func : annot → annot → annot.
+
+Lemma dec_eq_annot (x y : annot) : {x = y} + {x ≠ y}.
+Proof.
+  induction x in y |-*.
+  - destruct y; [now left| right; discriminate..].
+  - destruct y; [| now left |]; right; discriminate.
+  - destruct y; [right; discriminate..|].
+    destruct (IHx1 y1) as [-> | H].
+    + destruct (IHx2 y2) as [-> | H]; [now left|].
+      right.
+      now injection.
+    + right.
+      now injection.
+Qed.
+
+Lemma annot_UIP {x y : annot} (p q : x = y) : p = q.
+Proof.
+  apply Eqdep_dec.UIP_dec, dec_eq_annot.
+Qed.
+
+Fixpoint M_annot {n} (t : term n) : annot :=
+  match t with
+  | Srt _ => c
+  | Var _ => sing
+  | Abs _ t => M_annot t
+  | App t _ => M_annot t
+  | Pi ty fam =>
+      match M_annot fam with
+      | sing => sing
+      | ann_f =>
+          match M_annot ty with
+          | sing => ann_f
+          | ann_ty => func ann_ty ann_f
+          end
+      end
+  end.
+
+Fixpoint M_annot_ctx {m n} (K : ctx m n) (a : annot) : annot :=
+  match K with
+  | Hole => a 
+  | AbsL _ t => M_annot t
+  | AbsR _ K => M_annot_ctx K a
+  | AppL K _ => M_annot_ctx K a
+  | AppR t _ => M_annot t
+  | PiL K fam =>
+      match M_annot fam with
+      | sing => sing
+      | ann_f =>
+          match M_annot_ctx K a with
+          | sing => ann_f
+          | ann_ty => func ann_ty ann_f
+          end
+      end
+  | PiR ty K =>
+      match M_annot_ctx K a with
+      | sing => sing
+      | ann_f =>
+          match M_annot ty with
+          | sing => ann_f
+          | ann_ty => func ann_ty ann_f
+          end
+      end
+  end.
+
+Fixpoint ann_interp (ann : annot) : Prop :=
+  match ann with
+  | c => Cand
+  | sing => True
+  | func ann_b ann_f => ann_interp ann_b → ann_interp ann_f
+  end.
+
+Definition M {n} (t : term n) : Prop := ann_interp (M_annot t).
+
+Lemma M_annot_fill {m n} (t : term m) (K : ctx m n) :
+  M_annot (fill K t) = M_annot_ctx K (M_annot t).
+Proof.
+  induction K; auto;
+    simpl;
+    now rewrite IHK.
+Qed.
+
+Lemma M_annot_object {Sc n} (Γ : typing_ctx n) (t A : term n) :
+  Γ ⊢(Sc) A : Srt Star → Γ ⊢(Sc) t : A → M_annot t = sing.
+Proof.
+  induction 2; subst.
+  - contradict H.
+    clear.
+    remember (Srt Box).
+    induction 1; try discriminate; tauto.
+  - reflexivity.
+  - contradict H.
+    clear.
+    destruct s'; swap 1 2.
+    { remember (Srt Box).
+      induction 1; try discriminate; tauto.
+    }
+    intros C.
+    apply typ_star_inv in C.
+    apply srt_equiv_srt in C.
+    discriminate.
+  - simpl.
+    apply IHtyping3.
+    apply typ_pi_inv in H as (s1 & s2 & eq_star2 & typ_A & typ_B & pi_sc).
+    apply srt_equiv_srt in eq_star2.
+    subst.
+    assumption.
+  - simpl.
+    apply IHtyping1.
+    apply srt_typing in H0_ as [|[s' typ_piAB]]; [discriminate|].
+    apply typ_pi_inv in typ_piAB as (s1 & s2 & eq_star2 & typ_A & typ_B & pi_sc).
+    destruct s2; try solve [econstructor; eauto].
+    pose proof (bind_first_typ H0_0 typ_B) as typ_B'.
+    simpl in typ_B'.
+    pose proof (unique_typing H typ_B').
+    apply srt_equiv_srt in H0.
+    discriminate.
+  - apply IHtyping1.
+    apply srt_typing in H0_ as [C | [s' typ_C]].
+    + subst.
+      apply srt_equiv in H0.
+      pose proof (subject_reduction _ _ _ _ _ H H0) as C'.
+      contradict C'.
+      clear.
+      remember (Srt Box).
+      induction 1; try discriminate; tauto.
+    + destruct s'; [assumption|].
+      apply equiv_both_star in H0 as (v & red_A & red_B).
+      pose proof (subject_reduction _ _ _ _ _ typ_C red_A) as Hv1.
+      pose proof (subject_reduction _ _ _ _ _ H red_B) as Hv2.
+      pose proof (unique_typing Hv1 Hv2) as C''.
+      apply srt_equiv_srt in C''.
+      discriminate.
+Qed.
+
+Lemma M_annot_type {Sc n} (Γ : typing_ctx n) (A B : term n) :
+  Γ ⊢(Sc) B : Srt Box →
+  Γ ⊢(Sc) A : B → M_annot A = sing.
+Proof.
+  induction 2; subst; try discriminate.
+  - contradict H.
+    clear.
+    generalize (Srt (n := n) Box) at 2.
+    intros B.
+    remember (Srt Box).
+    induction 1; try discriminate; tauto.
+  - reflexivity.
+  - destruct s'; swap 1 2.
+    { contradict H.
+      clear.
+      generalize (Srt (n := n) Box) at 2.
+      intros B.
+      remember (Srt Box).
+      induction 1; try discriminate; tauto.
+    }
+    simpl.
+    rewrite IHtyping2; [reflexivity|].
+    constructor.
+    eapply typing_imp_ctx_wf.
+    eassumption.
+  - simpl.
+    apply IHtyping3.
+    apply typ_pi_inv in H as (s1 & s2 & eq_star2 & typ_A & typ_B & pi_sc).
+    apply srt_equiv_srt in eq_star2 as <-.
+    assumption.
+  - simpl.
+    apply IHtyping1.
+    apply srt_typing in H0_ as [|[s typ_B]]; [discriminate|].
+    apply typ_pi_inv in typ_B as (s1 & s2 & eq_star2 & typ_A & typ_B & pi_sc).
+    clear dependent s.
+    enough (s2 = Box).
+    + subst.
+      econstructor; eassumption.
+    + eapply srt_equiv_srt, unique_typing; [|eassumption].
+      eapply (bind_first_typ (T := Srt s2)); eassumption.
+ - apply IHtyping1.
+    apply srt_typing in H0_ as [C | [s' typ_C]].
+    + subst.
+      apply srt_equiv in H0.
+      pose proof (subject_reduction _ _ _ _ _ H H0) as C'.
+      contradict C'.
+      clear.
+      generalize (Srt (n := n) Box) at 2.
+      intros B.
+      remember (Srt Box).
+      induction 1; try discriminate; tauto.
+    + destruct s'; [|assumption].
+      apply equiv_both_star in H0 as (v & red_A & red_B).
+      pose proof (subject_reduction _ _ _ _ _ typ_C red_A) as Hv1.
+      pose proof (subject_reduction _ _ _ _ _ H red_B) as Hv2.
+      pose proof (unique_typing Hv1 Hv2) as C''.
+      apply srt_equiv_srt in C''.
+      discriminate.
+Qed.
+
+Lemma M_annot_typ_srt {Sc n} (Γ : typing_ctx n) (t A : term n) (s : sort):
+  Γ ⊢(Sc) A : Srt s →
+  Γ ⊢(Sc) t : A → M_annot t = sing.
+Proof.
+  destruct s.
+  - apply M_annot_object.
+  - apply M_annot_type.
+Qed.
+
+Lemma M_annot_ren {m} (t : term m) :
+  ∀ n (σ : {i | i < m} → {i | i < n}),
+  M_annot (ren σ t) = M_annot t.
+Proof.
+  induction t; simpl; trivial.
+  intros k σ.
+  rewrite IHt1, IHt2.
+  reflexivity.
+Qed.
+
+Lemma M_annot_bind {m} (t : term m) :
+  ∀ n (σ : {i | i < m} → term n),
+  (∀ i, M_annot (σ i) = sing) →
+  M_annot (bind σ t) = M_annot t.
+Proof.
+  induction t.
+  - simpl. auto.
+  - intros.
+    simpl.
+    rewrite IHt1, IHt2; trivial.
+    intros i.
+    unfold lift_bind.
+    destruct (lt_dec _ _).
+    + simpl.
+      now rewrite M_annot_ren.
+    + reflexivity.
+  - intros.
+    simpl.
+    apply IHt2.
+    unfold lift_bind.
+    intros.
+    destruct (lt_dec _ _).
+    + simpl.
+      now rewrite M_annot_ren.
+    + reflexivity.
+  - simpl. assumption.
+  - trivial.
+Qed.
+
+Lemma M_annot_head_step {Sc n} (Γ : typing_ctx n) (t u A B : term n) :
+  Γ ⊢(Sc) t : A →
+  t [≻] u →
+  M_annot t = M_annot u.
+Proof.
+  intros typ_t t_red.
+  destruct t_red.
+  simpl.
+  apply typ_app_inv in typ_t as (C & D & A_eq_B & typ_abs & typ_arg).
+  apply typ_abs_inv in typ_abs as (s1 & s2 & E & F & pi_eq & typ_ty & typ_E & typ_body & typ_pi & pi_sc).
+  apply pi_equiv_pi in pi_eq as [C_eq D_eq].
+  apply typ_pi_inv in typ_pi as (s3 & s4 & srt_eq & typ_C & typ_D & pi_sc').
+  symmetry.
+  apply M_annot_bind.
+  intros i.
+  unfold bind_first.
+  destruct (lt_dec _ _); [reflexivity|].
+  eapply M_annot_typ_srt; eassumption.
+Qed.
+
+Lemma M_annot_step {Sc n} (Γ : typing_ctx n) (t u A B : term n) :
+  Γ ⊢(Sc) t : A →
+  t ≻ u →
+  M_annot t = M_annot u.
+Proof.
+  intros typ_t red_t.
+  revert typ_t.
+  destruct red_t as [m K t' u' red_t'].
+  intros typ_Kt'.
+  rewrite !M_annot_fill.
+  f_equal.
+  apply typed_imp_subterm_typed in typ_Kt' as (Γ' & A' & typ_t').
+  eapply M_annot_head_step; eassumption.
+Qed.
+
+Lemma M_annot_red_plus {Sc n} (Γ : typing_ctx n) (t u A B : term n) :
+  Γ ⊢(Sc) t : A →
+  t ≻+ u →
+  M_annot t = M_annot u.
+Proof.
+  intros typ_t red_t.
+  induction red_t.
+  - rewrite IHred_t.
+    eapply M_annot_step; try eassumption.
+    eapply subject_reduction; [|apply Rclot_plus_star; eassumption].
+    eassumption.
+  - eapply M_annot_step; eassumption.
+Qed.
+
+Lemma M_annot_red {Sc n} (Γ : typing_ctx n) (t u A B : term n) :
+  Γ ⊢(Sc) t : A →
+  t ≻* u →
+  M_annot t = M_annot u.
+Proof.
+  intros typ_t red_t.
+  destruct red_t.
+  - reflexivity.
+  - eapply M_annot_red_plus; eassumption.
+Qed.
+
+Lemma M_annot_equiv {Sc n} (Γ Δ : typing_ctx n) (t u A B : term n) :
+  Γ ⊢(Sc) t : A →
+  Δ ⊢(Sc) u : B →
+  t ≅ u →
+  M_annot t = M_annot u.
+Proof.
+  intros typ_t typ_u t_eq_u.
+  apply equiv_both_star in t_eq_u as (v & red_t & red_u).
+  transitivity (M_annot v);
+    [|symmetry];
+    eapply M_annot_red;
+    eassumption.
+Qed.
+
+Lemma M_equiv {Sc n} (Γ Δ : typing_ctx n) (t u A B : term n) :
+  Γ ⊢(Sc) t : A →
+  Δ ⊢(Sc) u : B →
+  t ≅ u →
+  M t = M u.
+Proof.
+  intros.
+  unfold M.
+  f_equal.
+  eapply M_annot_equiv;
+    eassumption.
+Qed.
+
+Definition val (Sc : pi_scheme) {n} (Γ : typing_ctx n) :=
+  ∀ (i : nat) (H : i < n), M (kth_index_ctx Γ i H).
+
+Definition extend {Sc n} {Γ : typing_ctx n} {A} (Φ : val Sc Γ) (a : M A) : val Sc (Γ; A).
+Proof.
+  intros i H.
+  simpl kth_index_ctx.
+  unfold M. rewrite M_annot_ren.
+  destruct (lt_dec i n) as [H1 | H1].
+  - apply Φ.
+  - assumption.
+Defined.
+
+Fixpoint denot
+  Sc {n} (Γ : typing_ctx n)
+  (t A : term n) (H : Γ ⊢(Sc) t : A)
+  (Φ : val Sc Γ) {struct t}
+  : M A.
+Proof.
+  destruct t.
+  - apply typ_var_inv in H as A_eq_kth.
+    assert (e : M_annot A = M_annot (kth_index_ctx Γ (proj1_sig s) (proj2_sig s))).
+    {
+      apply srt_typing in H as typ_A.
+      apply typing_imp_ctx_wf in H.
+      destruct typ_A as [contra|[s' typ_A]].
+      + subst.
+        apply srt_equiv in A_eq_kth.
+        epose proof (wf_ctx_contains_types H) as [s' typ_kth].
+        eapply subject_reduction in typ_kth; [|eassumption].
+        contradict typ_kth.
+        clear.
+        remember (Srt Box) as B.
+        induction 1; try discriminate; tauto.
+      + epose proof (wf_ctx_contains_types H) as [s'' typ_kth].
+        eapply M_annot_equiv; try eassumption.
+    }
+    unfold M.
+    rewrite e.
+    apply Φ.
+  - apply typ_pi_inv in H as H1.
+    destruct H1 as (s & s' & A_eq_s' & typ_t1 & typ_t2 & psc).
+    assert (M_annot A = c).
+    {
+      destruct s'.
+      - apply srt_typing in H as [contra|typ_A].
+        { subst.
+          now apply srt_equiv_srt in A_eq_s'.
+        }
+        destruct typ_A as [s0 typ_A].
+        unshelve erewrite (M_annot_equiv _ _ _ _ _ _ _ ltac:(constructor) A_eq_s').
+        5 : eassumption.
+        1 : assumption.
+        { eapply typing_imp_ctx_wf. eassumption. }
+        reflexivity.
+      - apply Requiv_sym, srt_equiv in A_eq_s'.
+        apply srt_typing in H as [|[s0 typ_A]]; [now subst|].
+        pose proof (subject_reduction _ _ _ _ _ typ_A A_eq_s') as C'.
+        contradict C'.
+        clear.
+        remember (Srt Box).
+        induction 1; try discriminate; tauto.
+    }
+    unfold M.
+    rewrite H0.
+    set (X := denot _ _ _ _ _ typ_t1 Φ).
+    destruct X as [X cX].
+    set (S := λ (Y : tset), ∃ c H, ex_intro _ Y H = denot Sc _ _ t2 _ typ_t2 (extend Φ c)).
+    econstructor.
+    unshelve eapply (c_pi _ S _ _ cX).
+    { apply tset_equiv_refl. }
+    intros Y HY.
+    unfold S, elem in HY.
+    now destruct HY as (c & cY & Y_eq).
+  - apply typ_abs_inv in H as H1.
+    destruct H1 as (s & s' & B & X & A_eq & typ_t1 & typ_B & typ_t2 & typ_1 & psc).
+    unfold M.
+    unshelve erewrite (M_annot_equiv _ Γ _ _ _ _ typ_1 _ A_eq).
+    2 : {econstructor; eassumption. }
+    simpl.
+    assert (M_annot B = sing ∨ M_annot B ≠ sing) as [-> | ann_B].
+    {
+      destruct (M_annot B); [now left|right..]; discriminate.
+    }
+    { now simpl. }
+    assert (M_annot t1 = sing ∨ M_annot t1 ≠ sing) as [ann_t1 | ann_t1].
+    {
+      destruct (M_annot t1); [now left|right..]; discriminate.
+    }
+    {
+      assert (e : M t1).
+      {
+        unfold M.
+        rewrite ann_t1.
+        now simpl.
+      }
+      rewrite ann_t1.
+      pose proof (v := denot _ _ _ _ _ typ_t2 (extend Φ e)).
+      unfold M in v.
+      now destruct (M_annot B) eqn:ann_B'.
+    }
+    pose proof (λ x, denot _ _ _ _ _ typ_t2 (extend Φ x)) as f.
+    unfold M in f.
+    destruct (M_annot B), (M_annot t1); try contradiction; assumption.
+  - apply typ_app_inv in H as H1.
+    destruct H1 as (A0 & B & A_eq & typ_t1 & typ_t2).
+    apply srt_typing in typ_t1 as H2.
+    destruct H2 as [|[s0 H2]]; [discriminate|].
+    apply typ_pi_inv in H2 as H3.
+    destruct H3 as (s & s' & srt_eq & typ_A0 & typ_B & psc).
+    apply srt_equiv_srt in srt_eq as ->.
+    assert (M_annot t2 = sing).
+    {
+      eapply M_annot_typ_srt; eassumption.
+    }
+    unfold M.
+    replace (M_annot A) with (M_annot B); swap 1 2.
+    {
+      apply srt_typing in H as [-> | [s0 H1]].
+      { eapply srt_equiv, subject_reduction in A_eq; swap 1 2.
+        - eapply bind_first_typ; eassumption.
+        - simpl in A_eq.
+          contradict A_eq.
+          clear.
+          remember (Srt Box).
+          induction 1; try discriminate; tauto.
+      }
+      unshelve erewrite (M_annot_equiv _ _ _ _ _ _ _ _ A_eq).
+      7 : { eapply bind_first_typ; eassumption. }
+      3 : { apply H1. }
+      symmetry.
+      apply M_annot_bind.
+      intros i.
+      unfold bind_first.
+      now destruct (lt_dec _ _).
+    }
+    pose proof (denot _ _ _ _ _ typ_t1 Φ) as f.
+    pose proof (denot _ _ _ _ _ typ_t2 Φ) as x.
+    unfold M in f, x.
+    simpl in f.
+    assert (M_annot B = sing ∨ M_annot B ≠ sing) as [-> | ann_B].
+    {
+      destruct (M_annot B); [now left|right..]; discriminate.
+    }
+    { now simpl. }
+    assert (M_annot A0 = sing ∨ M_annot A0 ≠ sing) as [ann_A0 | ann_A0].
+    {
+      destruct (M_annot A0); [now left|right..]; discriminate.
+    }
+    { rewrite ann_A0 in *.
+      now destruct (M_annot B).
+    }
+    destruct (M_annot A0), (M_annot B); try contradiction; exact (f x).
+  - destruct s.
+    + apply srt_typing in H as H1.
+      destruct H1 as [->|contra].
+      { exact cand_sn. }
+      destruct contra as [s0 H1].
+      apply typ_star_inv, Requiv_sym, srt_equiv in H.
+      eapply subject_reduction in H1; [|eassumption].
+      contradict H1.
+      clear.
+      remember (Srt Box).
+      induction 1; try discriminate; tauto.
+    + contradict H.
+      clear.
+      remember (Srt Box).
+      induction 1; try discriminate; tauto.
+Defined.
+
+Lemma denot_irrel
+  Sc {n} (Γ : typing_ctx n)
+  (t A : term n) (H1 H2 : Γ ⊢(Sc) t : A)
+  (Φ : val Sc Γ) : denot _ _ _ _ H1 Φ = denot _ _ _ _ H2 Φ.
+Proof.
+  induction t; simpl.
+  - f_equal.
+    apply annot_UIP.
+  - destruct (typ_pi_inv _ _ _ _ _), (typ_pi_inv _ _ _ _ _).
+    destruct e, e0.
+    destruct a, a0.
+    destruct a, a0.
+    destruct a, a0.
+    f_equal.
+    + assert (x = x0) as q.
+      {
+        eapply srt_equiv_srt, unique_typing; eassumption.
+      }
+      destruct q.
+      assert (x1 = x2) as q.
+      {
+        eapply srt_equiv_srt, unique_typing; eassumption.
+      }
+      destruct q.
+      rewrite (IHt1 _ _ t t0).
+      destruct (denot _ _ _ _ _).
+      unshelve eapply eq_ex_intro.
+      * f_equal.
+     (* Unfortunately this requires funext, stating a
+        precise equivalence lemma might be too involved*)
+Abort. 
+
 
 Lemma typing_SN {Sc : pi_scheme} {n : nat} (Γ : typing_ctx n) (t A : term n) :
   Γ ⊢(Sc) t : A → SN t.
